@prefix : <https://cogito.iot.linkeddata.es/quality#> .
@prefix owl: <http://www.w3.org/2002/07/owl#> .
@prefix rdf: <http://www.w3.org/1999/02/22-rdf-syntax-ns#> .
@prefix xml: <http://www.w3.org/XML/1998/namespace> .
@prefix xsd: <http://www.w3.org/2001/XMLSchema#> .
@prefix qual: <https://cogito.iot.linkeddata.es/quality#> .
@prefix rdfs: <http://www.w3.org/2000/01/rdf-schema#> .
@prefix saref: <https://saref.etsi.org/core#> .
@prefix dcterms: <http://purl.org/dc/terms/> .
@prefix process: <https://cogito.iot.linkeddata.es/process#> .
@prefix facility: <https://cogito.iot.linkeddata.es/def/facility#> .
@base <https://cogito.iot.linkeddata.es/quality#> .

<https://cogito.iot.linkeddata.es/quality#> rdf:type owl:Ontology ;
                                             <http://purl.org/dc/elements/1.1/creator> "María Poveda Villalón" ,
                                                                                       "Raúl García Castro" ,
                                                                                       "Socorro  Bernardos Galindo" ;
                                             <http://purl.org/dc/elements/1.1/description> "The COGITO Quality ontology aims at modelling the construction quality domain." ;
                                             <http://purl.org/dc/elements/1.1/title> "Quality Ontology" ;
                                             dcterms:license <http://purl.org/NET/rdflicense/cc-by4.0> ;
                                             owl:versionInfo "0.12.0" .

#################################################################
#    Annotation properties
#################################################################

###  http://purl.org/dc/elements/1.1/creator
<http://purl.org/dc/elements/1.1/creator> rdf:type owl:AnnotationProperty .


###  http://purl.org/dc/elements/1.1/description
<http://purl.org/dc/elements/1.1/description> rdf:type owl:AnnotationProperty .


###  http://purl.org/dc/elements/1.1/title
<http://purl.org/dc/elements/1.1/title> rdf:type owl:AnnotationProperty .


###  http://purl.org/dc/terms/license
dcterms:license rdf:type owl:AnnotationProperty .


#################################################################
#    Object Properties
#################################################################

###  https://cogito.iot.linkeddata.es/def/quality#isRelatedToProject
<https://cogito.iot.linkeddata.es/def/quality#isRelatedToProject> rdf:type owl:ObjectProperty ;
                                                                  rdfs:range facility:Project ;
                                                                  rdfs:comment "Property that relates an entity (especially qual:QualityInformation and quel:Rule) to a facility:Project" ;
                                                                  rdfs:label "is related to project" .


###  https://cogito.iot.linkeddata.es/quality#hasInformationResource
qual:hasInformationResource rdf:type owl:ObjectProperty ;
                            owl:inverseOf qual:isRelatedToElement ;
                            rdfs:range qual:InformationResource ;
                            rdfs:comment "Property that relates an entity (especially a facility:Element) to a qual:InformationResource" ;
                            rdfs:label "has information resource" .


###  https://cogito.iot.linkeddata.es/quality#hasProcessedImage
qual:hasProcessedImage rdf:type owl:ObjectProperty ;
                       rdfs:range qual:Image ;
                       rdfs:comment "Property that relates an entity (especially qual:ImageJob to a processed qual:Image" ;
                       rdfs:label "has processed image" .


###  https://cogito.iot.linkeddata.es/quality#hasRawImage
qual:hasRawImage rdf:type owl:ObjectProperty ;
                 rdfs:subPropertyOf owl:topObjectProperty ;
                 owl:inverseOf qual:isRelatedToJob ;
                 rdfs:range qual:RawImage ;
                 rdfs:comment "Property that relates an entity (especially qual:ImageJob to an original qual:Image" ;
                 rdfs:label "has raw image" .


###  https://cogito.iot.linkeddata.es/quality#hasResultImage
qual:hasResultImage rdf:type owl:ObjectProperty ;
                    rdfs:range qual:Image ;
                    rdfs:comment "Property that relates an entity (especially qual:ImageJob to a resulting qual:Image" ;
                    rdfs:label "has result image" .


###  https://cogito.iot.linkeddata.es/quality#isRelatedToElement
qual:isRelatedToElement rdf:type owl:ObjectProperty ;
                        rdfs:range facility:Element ;
                        rdfs:comment "Property that relates an entity (especially qual:InformationResource) to a facility:Element" ;
                        rdfs:label "is related to element" .


###  https://cogito.iot.linkeddata.es/quality#isRelatedToJob
qual:isRelatedToJob rdf:type owl:ObjectProperty ;
                    rdfs:comment "Property that relates an entity (especially a qual:RawImage) to the qual:ImageJob that it is associated to" ;
                    rdfs:label "is related to job" .


###  https://cogito.iot.linkeddata.es/quality#isRelatedToTask
qual:isRelatedToTask rdf:type owl:ObjectProperty ;
                     rdfs:range process:Task ;
                     rdfs:comment "Property that relates an entity (especially qual:QuqlityInformation and qual:QualityInformation) to a process:Task" ;
                     rdfs:label "is related to task" .


###  https://cogito.iot.linkeddata.es/quality#isTheResultToJob
qual:isTheResultToJob rdf:type owl:ObjectProperty ;
                      owl:inverseOf qual:producesVisualQualityInformation ;
                      rdfs:comment "Property that relates an entity (especially a qual:VisualQualityInformation ) to the qual:ImageJob that has produced it" ;
                      rdfs:label "is the result to job" .


###  https://cogito.iot.linkeddata.es/quality#producesGeometricQualityInformation
qual:producesGeometricQualityInformation rdf:type owl:ObjectProperty ;
                                         rdfs:subPropertyOf qual:producesQualityInformation ;
                                         rdfs:range qual:GeometricQualityInformation ;
                                         rdfs:comment "Property that relates an entity (especially a qual:PointCloud) to the qual:GeometricQualityInformation it produces" ;
                                         rdfs:label "produces geometric quality information" .


###  https://cogito.iot.linkeddata.es/quality#producesQualityInformation
qual:producesQualityInformation rdf:type owl:ObjectProperty ;
                                rdfs:comment "Property that relates an entity (especially a qual:InformationResource) to the qual:QualityInformation it produces." ;
                                rdfs:label "produces quality information" .


###  https://cogito.iot.linkeddata.es/quality#producesVisualQualityInformation
qual:producesVisualQualityInformation rdf:type owl:ObjectProperty ;
                                      rdfs:subPropertyOf qual:producesQualityInformation ;
                                      rdfs:range qual:VisualQualityInformation ;
                                      rdfs:comment "Property that relates an entity (especially a qual:ImageJob) to the qual:VisualQualityInformation it produces" ;
                                      rdfs:label "produces visual quality information" .


###  https://cogito.iot.linkeddata.es/quality#refersToElement
qual:refersToElement rdf:type owl:ObjectProperty ;
                     rdfs:range facility:Element ;
                     rdfs:comment "Property that relates an entity (especially qual:QualityResult) to a facility:Element" ;
                     rdfs:label "refers to element" .


###  https://cogito.iot.linkeddata.es/quality#refersToGeometricQualityInf
qual:refersToGeometricQualityInf rdf:type owl:ObjectProperty ;
                                 rdfs:range qual:GeometricQualityInformation ;
                                 rdfs:comment "Property that relates an entity (especially a facility:Element) to a qual:GeometricQualityInformation" ;
                                 rdfs:label "refers to geometric quality information" .


###  https://cogito.iot.linkeddata.es/quality#refersToRule
qual:refersToRule rdf:type owl:ObjectProperty ;
                  rdfs:range qual:Rule ;
                  rdfs:comment "Property that relates an entity (especially qual:Defect) to a qual:Rule" ;
                  rdfs:label "refers to rule" .


#################################################################
#    Data properties
#################################################################

###  http://purl.org/dc/terms/description
dcterms:description rdf:type owl:DatatypeProperty ;
                    rdfs:isDefinedBy dcterms: ;
                    rdfs:label "description" .


###  http://purl.org/dc/terms/identifier
dcterms:identifier rdf:type owl:DatatypeProperty ;
                   rdfs:isDefinedBy dcterms: ;
                   rdfs:label "identifier" .


###  http://purl.org/dc/terms/title
dcterms:title rdf:type owl:DatatypeProperty ;
              rdfs:isDefinedBy dcterms: ;
              rdfs:label "title" .


###  https://cogito.iot.linkeddata.es/quality#captureDevice
qual:captureDevice rdf:type owl:DatatypeProperty ;
                   rdfs:comment "Property identifying  the device that has captured an entity (especially a qual:Image)" ;
                   rdfs:label "capture device" .


###  https://cogito.iot.linkeddata.es/quality#confidenceLevel
qual:confidenceLevel rdf:type owl:DatatypeProperty ;
                     rdfs:comment "Property indicating the level of confidence of a result (especially a qual:Defect)" ;
                     rdfs:label "confidence level" .


###  https://cogito.iot.linkeddata.es/quality#deviceOrientation
qual:deviceOrientation rdf:type owl:DatatypeProperty ;
                       rdfs:comment "Property indicating the orientation of a device" ;
                       rdfs:label "device orientation" .


###  https://cogito.iot.linkeddata.es/quality#devicePosition
qual:devicePosition rdf:type owl:DatatypeProperty ;
                    rdfs:comment "Property indication the position of a device" ;
                    rdfs:label "device position" .


###  https://cogito.iot.linkeddata.es/quality#elementTypeKeyword
qual:elementTypeKeyword rdf:type owl:DatatypeProperty ;
                        rdfs:comment "List of keywords related to the element type" ;
                        rdfs:label "element type keywords" .


###  https://cogito.iot.linkeddata.es/quality#materialTypeKeyword
qual:materialTypeKeyword rdf:type owl:DatatypeProperty ;
                         rdfs:comment "List of keywords related to the material type" ;
                         rdfs:label "material type keywords" .


###  https://cogito.iot.linkeddata.es/quality#originDocument
qual:originDocument rdf:type owl:DatatypeProperty ;
                    rdfs:comment "Property indicating the origin document of an entity (especially a qual:GeometricQualityInformation)" ;
                    rdfs:label "origin document" .


###  https://cogito.iot.linkeddata.es/quality#outcome
qual:outcome rdf:type owl:DatatypeProperty ;
             rdfs:comment "Property indicating if a result has been accepted or rejected" ;
             rdfs:label "outcome" .


###  https://cogito.iot.linkeddata.es/quality#performedTimestamp
qual:performedTimestamp rdf:type owl:DatatypeProperty ;
                        rdfs:comment "Property indicating the actual time an entity has been performed" ;
                        rdfs:label "performed timestamp" .


###  https://cogito.iot.linkeddata.es/quality#predictedLabel
qual:predictedLabel rdf:type owl:DatatypeProperty ;
                    rdfs:comment "Property indicating the origin document of an entity (especially a qual:Defect)" ;
                    rdfs:label "predicted label" .


###  https://cogito.iot.linkeddata.es/quality#relationshipTypeKeyword
qual:relationshipTypeKeyword rdf:type owl:DatatypeProperty ;
                             rdfs:comment "List of keywords related to the relationship type" ;
                             rdfs:label "relationship type keywords" .


###  https://cogito.iot.linkeddata.es/quality#result
qual:result rdf:type owl:DatatypeProperty ;
            rdfs:comment "Property indicating the result of an entity (especially a qual:GeometricQualityInformation" ;
            rdfs:label "result" .


###  https://cogito.iot.linkeddata.es/quality#scalarResult
qual:scalarResult rdf:type owl:DatatypeProperty ;
                  rdfs:comment "Property indicating the scalar result" ;
                  rdfs:label "scalar result" .


###  https://cogito.iot.linkeddata.es/quality#scheduledTimestamp
qual:scheduledTimestamp rdf:type owl:DatatypeProperty ;
                        rdfs:comment "Property indicating the scheduled time" ;
                        rdfs:label "scheduled timestamp" .


###  https://cogito.iot.linkeddata.es/quality#severity
qual:severity rdf:type owl:DatatypeProperty ;
              rdfs:comment "A property indicating the severity of an entity (especially a qual:Defect)" ;
              rdfs:label "severity" .


###  https://cogito.iot.linkeddata.es/quality#status
qual:status rdf:type owl:DatatypeProperty ;
            rdfs:comment "Property indicating if a result has been checked" ;
            rdfs:label "status" .


###  https://cogito.iot.linkeddata.es/quality#takenAtTime
qual:takenAtTime rdf:type owl:DatatypeProperty ;
                 rdfs:comment "Property indicating the time a data has been taken" ;
                 rdfs:label "taken at time" .


###  https://cogito.iot.linkeddata.es/quality#toleranceReference
qual:toleranceReference rdf:type owl:DatatypeProperty ;
                        rdfs:comment "property indicating the tolerance reference" ;
                        rdfs:label "tolerance reference" .


###  https://cogito.iot.linkeddata.es/quality#unit
qual:unit rdf:type owl:DatatypeProperty ;
          rdfs:comment "Property indicating the unit of an entity" ;
          rdfs:label "unit" .


###  https://cogito.iot.linkeddata.es/quality#uploadedTimestamp
qual:uploadedTimestamp rdf:type owl:DatatypeProperty ;
                       rdfs:comment "Property indicating the actual time an entity has been uploaded" ;
                       rdfs:label "uploaded timestamp" .


#################################################################
#    Classes
#################################################################

###  https://cogito.iot.linkeddata.es/def/facility#Element
facility:Element rdf:type owl:Class ;
                 rdfs:comment "A subclass or bot:Element and, as such, a constituent of a construction entity with a characteristic technical function, form, or position" ;
                 rdfs:label "Element" .


###  https://cogito.iot.linkeddata.es/def/facility#Project
facility:Project rdf:type owl:Class ;
                 rdfs:comment "A large or major undertaking, especially one involving considerable money, personnel, and equipment" ;
                 rdfs:label "Project" .


###  https://cogito.iot.linkeddata.es/process#Task
process:Task rdf:type owl:Class ;
             rdfs:comment "A piece of work, which is performed in a process:Process" ;
             rdfs:label "Task" .


###  https://cogito.iot.linkeddata.es/quality#AsBuiltMesh
qual:AsBuiltMesh rdf:type owl:Class ;
                 rdfs:subClassOf qual:Mesh ;
                 rdfs:comment "A mesh representing a built entity (especially a facility:Element)" ;
                 rdfs:label "As-built Mesh" .


###  https://cogito.iot.linkeddata.es/quality#AsBuiltPointCloud
qual:AsBuiltPointCloud rdf:type owl:Class ;
                       rdfs:subClassOf qual:PointCloud ;
                       rdfs:comment "A point cloud representing a built entity (especially a facility:Element)" ;
                       rdfs:label "As-built Point Cloud" .


###  https://cogito.iot.linkeddata.es/quality#GeometricQualityInformation
qual:GeometricQualityInformation rdf:type owl:Class ;
                                 rdfs:subClassOf qual:QualityInformation ;
                                 rdfs:comment "Data informing a particular problem regarding a particular qual:Rule on a facility:Element, and found thanks to a process:GeometricQualityTask" ;
                                 rdfs:label "Geometric Quality Information" .


###  https://cogito.iot.linkeddata.es/quality#Image
qual:Image rdf:type owl:Class ;
           rdfs:subClassOf qual:InformationResource ;
           rdfs:comment "A picture of an entity" ;
           rdfs:label "Image" .


###  https://cogito.iot.linkeddata.es/quality#ImageJob
qual:ImageJob rdf:type owl:Class ;
              rdfs:subClassOf qual:InformationResource ;
              rdfs:comment "Data regarding an image and the results of processing it" ;
              rdfs:label "Image Job" .


###  https://cogito.iot.linkeddata.es/quality#InformationResource
qual:InformationResource rdf:type owl:Class ;
                         rdfs:comment "Data regarding  the quality of an entity (especially a facility:Project or facility:Element) and that may have associated files in the platform" ;
                         rdfs:label "Quality Information" .


###  https://cogito.iot.linkeddata.es/quality#Mesh
qual:Mesh rdf:type owl:Class ;
          rdfs:subClassOf qual:InformationResource ;
          rdfs:comment "A collection of vertices, edges and faces that defines the shape of an object (especially a facility:Element)" ;
          rdfs:label "Mesh" .


###  https://cogito.iot.linkeddata.es/quality#PointCloud
qual:PointCloud rdf:type owl:Class ;
                rdfs:subClassOf qual:InformationResource ;
                rdfs:comment "A set of data points in space" ;
                rdfs:label "Point Cloud" .


###  https://cogito.iot.linkeddata.es/quality#QualityInformation
qual:QualityInformation rdf:type owl:Class ;
                        rdfs:comment "The result of the analysis of  information (especially qual:QuantityInformation)" ;
                        rdfs:label "Quality Information" .


###  https://cogito.iot.linkeddata.es/quality#RawImage
qual:RawImage rdf:type owl:Class ;
              rdfs:subClassOf qual:Image ;
              rdfs:comment "An image that has not been processed" ;
              rdfs:label "Raw Image" .


###  https://cogito.iot.linkeddata.es/quality#Rule
qual:Rule rdf:type owl:Class ;
          rdfs:comment "Information regarding what an entity (especially a faciity:Element) must fulfil" ;
          rdfs:label "Rule" .


###  https://cogito.iot.linkeddata.es/quality#VisualQualityInformation
qual:VisualQualityInformation rdf:type owl:Class ;
                              rdfs:subClassOf qual:QualityInformation ;
                              rdfs:comment "A shortcoming, fault, or imperfection regarding a particular facility:Element, and found thanks to a process:VisualQualityTask" ;
                              rdfs:label "Visual Quality Information" .


###  Generated by the OWL API (version 4.5.9.2019-02-01T07:24:44Z) https://github.com/owlcs/owlapi
